Rename fix_mutrec, fix_rec -> mrec, rec

theories/Fix.v
@@ -50,11 +50,11 @@ From ITree Require Import
      end.
 ]]
 
-   The function [interp_mutrec] below then ties the knot.
+   The function [interp_mrec] below then ties the knot.
 
 [[
    Definition f : D ~> itree emptyE :=
-     interp_mutrec def.
+     interp_mrec def.
 
    Definition even (n : nat) : itree emptyE bool := f _ (Even n).
    Definition odd  (n : nat) : itree emptyE bool := f _ (Odd n).
@@ -68,7 +68,7 @@ From ITree Require Import
 
 (** Interpret an itree in the context of a mutually recursive
     definition ([ctx]). *)
-Definition interp_mutrec {D E : Type -> Type}
+Definition interp_mrec {D E : Type -> Type}
            (ctx : D ~> itree (D +' E)) : itree (D +' E) ~> itree E :=
   fun R =>
     cofix mutfix_ (t : itree (D +' E) R) : itree E R :=
@@ -78,9 +78,9 @@ Definition interp_mutrec {D E : Type -> Type}
 
 (** Unfold a mutually recursive definition into separate trees,
     resolving the mutual references. *)
-Definition fix_mutrec {D E : Type -> Type}
+Definition mrec {D E : Type -> Type}
            (ctx : D ~> itree (D +' E)) : D ~> itree E :=
-  fun R d => interp_mutrec ctx _ (ctx _ d).
+  fun R d => interp_mrec ctx _ (ctx _ d).
 
 Inductive callE (A B : Type) : Type -> Type :=
 | Call : A -> callE A B B.
@@ -88,66 +88,66 @@ Inductive callE (A B : Type) : Type -> Type :=
 Arguments Call {A B}.
 
 (* Interpret a single recursive definition. *)
-Definition fix_rec {E : Type -> Type} {A B : Type}
+Definition rec {E : Type -> Type} {A B : Type}
            (body : A -> itree (callE A B +' E) B) :
   A -> itree E B :=
-  fun a => fix_mutrec (fun _ call =>
+  fun a => mrec (fun _ call =>
     match call in callE _ _ T return itree (_ +' E) T with
     | Call a => body a
     end) _ (Call a).
 
-(** Properties of [interp_mutrec] and [fix_mutrec]. *)
+(** Properties of [interp_mrec] and [mrec]. *)
 Section Facts.
 
 Context {D E : Type -> Type} (ctx : D ~> itree (D +' E)).
 
-(** Unfolding of [interp_mutrec]. *)
-Definition interp_mutrecF R :
+(** Unfolding of [interp_mrec]. *)
+Definition interp_mrecF R :
   itreeF (D +' E) R _ -> itree E R :=
-  handleF1 (interp_mutrec ctx R)
-           (fun _ d k => Tau (interp_mutrec ctx _ (ctx _ d >>= k))).
+  handleF1 (interp_mrec ctx R)
+           (fun _ d k => Tau (interp_mrec ctx _ (ctx _ d >>= k))).
 
-Lemma unfold_interp_mutrecF R (t : itree (D +' E) R) :
-  observe (interp_mutrec ctx _ t) = observe (interp_mutrecF _ (observe t)).
+Lemma unfold_interp_mrecF R (t : itree (D +' E) R) :
+  observe (interp_mrec ctx _ t) = observe (interp_mrecF _ (observe t)).
 Proof. reflexivity. Qed.
 
-Lemma unfold_interp_mutrec R (t : itree (D +' E) R) :
-  eq_itree (interp_mutrec ctx _ t)
-           (interp_mutrecF _ (observe t)).
+Lemma unfold_interp_mrec R (t : itree (D +' E) R) :
+  eq_itree (interp_mrec ctx _ t)
+           (interp_mrecF _ (observe t)).
 Proof.
-  rewrite itree_eta, unfold_interp_mutrecF, <-itree_eta.
+  rewrite itree_eta, unfold_interp_mrecF, <-itree_eta.
   reflexivity.
 Qed.
 
-Lemma ret_mutrec {T} (x: T) :
-  interp_mutrec ctx _ (Ret x) ≅ Ret x.
-Proof. rewrite unfold_interp_mutrec; reflexivity. Qed.
+Lemma ret_mrec {T} (x: T) :
+  interp_mrec ctx _ (Ret x) ≅ Ret x.
+Proof. rewrite unfold_interp_mrec; reflexivity. Qed.
 
-Lemma tau_mutrec {T} (t: itree _ T) :
-  interp_mutrec ctx _ (Tau t) ≅ Tau (interp_mutrec ctx _ t).
-Proof. rewrite unfold_interp_mutrec. reflexivity. Qed.
+Lemma tau_mrec {T} (t: itree _ T) :
+  interp_mrec ctx _ (Tau t) ≅ Tau (interp_mrec ctx _ t).
+Proof. rewrite unfold_interp_mrec. reflexivity. Qed.
 
-Lemma vis_mutrec_right {T U} (e : E U) (k : U -> itree (D +' E) T) :
-  interp_mutrec ctx _ (Vis (inr1 e) k) ≅
-  Vis e (fun x => interp_mutrec ctx _ (k x)).
-Proof. rewrite unfold_interp_mutrec. reflexivity. Qed.
+Lemma vis_mrec_right {T U} (e : E U) (k : U -> itree (D +' E) T) :
+  interp_mrec ctx _ (Vis (inr1 e) k) ≅
+  Vis e (fun x => interp_mrec ctx _ (k x)).
+Proof. rewrite unfold_interp_mrec. reflexivity. Qed.
 
-Lemma vis_mutrec_left {T U} (d : D U) (k : U -> itree (D +' E) T) :
-  interp_mutrec ctx _ (Vis (inl1 d) k) ≅
-  Tau (interp_mutrec ctx _ (ITree.bind (ctx _ d) k)).
-Proof. rewrite unfold_interp_mutrec. reflexivity. Qed.
+Lemma vis_mrec_left {T U} (d : D U) (k : U -> itree (D +' E) T) :
+  interp_mrec ctx _ (Vis (inl1 d) k) ≅
+  Tau (interp_mrec ctx _ (ITree.bind (ctx _ d) k)).
+Proof. rewrite unfold_interp_mrec. reflexivity. Qed.
 
-Hint Rewrite @ret_mutrec : itree.
-Hint Rewrite @vis_mutrec_left : itree.
-Hint Rewrite @vis_mutrec_right : itree.
-Hint Rewrite @tau_mutrec : itree.
+Hint Rewrite @ret_mrec : itree.
+Hint Rewrite @vis_mrec_left : itree.
+Hint Rewrite @vis_mrec_right : itree.
+Hint Rewrite @tau_mrec : itree.
 
-Instance eq_itree_mutrec {R} :
-  Proper (@eq_itree _ R ==> @eq_itree _ R) (interp_mutrec ctx R).
+Instance eq_itree_mrec {R} :
+  Proper (@eq_itree _ R ==> @eq_itree _ R) (interp_mrec ctx R).
 Proof.
   repeat intro. pupto2_init. revert_until R.
   pcofix CIH. intros.
-  rewrite !unfold_interp_mutrec.
+  rewrite !unfold_interp_mrec.
   pupto2_final.
   punfold H0. inv H0; pclearbot; [| |destruct e].
   - eapply eq_itree_refl.
@@ -157,9 +157,9 @@ Proof.
   - pfold. econstructor. eauto 7.
 Qed.
 
-Theorem interp_mutrec_bind {U T} (t : itree _ U) (k : U -> itree _ T) :
-  interp_mutrec ctx _ (ITree.bind t k) ≅
-  ITree.bind (interp_mutrec ctx _ t) (fun x => interp_mutrec ctx _ (k x)).
+Theorem interp_mrec_bind {U T} (t : itree _ U) (k : U -> itree _ T) :
+  interp_mrec ctx _ (ITree.bind t k) ≅
+  ITree.bind (interp_mrec ctx _ t) (fun x => interp_mrec ctx _ (k x)).
 Proof.
   intros. pupto2_init. revert t k.
   pcofix CIH. intros.
@@ -173,86 +173,86 @@ Proof.
   all: try (pfold; econstructor; eauto).
 Qed.
 
-Let h_mutrec : D ~> itree E := fix_mutrec ctx.
+Let h_mrec : D ~> itree E := mrec ctx.
 
-Inductive mutrec_invariant {U} : relation (itree _ U) :=
-| mutrec_main (d1 d2 : _ U) (Ed : eq_itree d1 d2) :
-    mutrec_invariant (interp_mutrec ctx _ d1)
-                     (interp1 (fix_mutrec ctx) _ d2)
-| mutrec_bind T (d : _ T) (k1 k2 : T -> itree _ U)
+Inductive mrec_invariant {U} : relation (itree _ U) :=
+| mrec_main (d1 d2 : _ U) (Ed : eq_itree d1 d2) :
+    mrec_invariant (interp_mrec ctx _ d1)
+                     (interp1 (mrec ctx) _ d2)
+| mrec_bind T (d : _ T) (k1 k2 : T -> itree _ U)
     (Ek : forall x, eq_itree (k1 x) (k2 x)) :
-    mutrec_invariant (interp_mutrec ctx _ (d >>= k1))
-                     (interp_mutrec ctx _ d >>= fun x =>
-                        interp1 h_mutrec _ (k2 x))
+    mrec_invariant (interp_mrec ctx _ (d >>= k1))
+                     (interp_mrec ctx _ d >>= fun x =>
+                        interp1 h_mrec _ (k2 x))
 .
 
 Notation mi_holds r :=
   (forall c1 c2 d1 d2,
-      mutrec_invariant d1 d2 ->
+      mrec_invariant d1 d2 ->
       eq_itree c1 d1 -> eq_itree c2 d2 -> r c1 c2).
 
-Lemma mutrec_invariant_init {U} (r : relation (itree _ U))
+Lemma mrec_invariant_init {U} (r : relation (itree _ U))
       (INV : mi_holds r)
       (c1 c2 : itree _ U)
       (Ec : eq_itree c1 c2) :
   paco2 (compose eq_itreeF (gres2 eq_itreeF)) r
-        (interp_mutrec ctx _ c1)
-        (interp1 h_mutrec _ c2).
+        (interp_mrec ctx _ c1)
+        (interp1 h_mrec _ c2).
 Proof.
-  rewrite unfold_interp_mutrec, unfold_interp1.
+  rewrite unfold_interp_mrec, unfold_interp1.
   punfold Ec.
   inversion Ec; cbn; pclearbot; pupto2_final.
   + eapply eq_itree_refl. (* This should be reflexivity. *)
   + pfold; constructor. right; eapply INV.
-    1: apply mutrec_main; eassumption.
+    1: apply mrec_main; eassumption.
     all: reflexivity.
   + destruct e.
     { pfold; constructor; cbn; right. eapply INV.
-      1: apply mutrec_bind; eassumption.
+      1: apply mrec_bind; eassumption.
       all: cbn; reflexivity.
     }
     { pfold; econstructor.
       intros; right. eapply INV.
-      1: apply mutrec_main; eapply REL.
+      1: apply mrec_main; eapply REL.
       all: reflexivity.
     }
 Qed.
 
-Lemma mutrec_invariant_eq {U} : mi_holds (@eq_itree _ U).
+Lemma mrec_invariant_eq {U} : mi_holds (@eq_itree _ U).
 Proof.
   intros d1 d2 c1 c2 Ec1 Ec2 H.
   pupto2_init; revert d1 d2 c1 c2 Ec1 Ec2 H; pcofix self.
   intros _d1 _d2 c1 c2 [d1 d2 Ed | T d k1 k2 Ek] Ec1 Ec2.
   - rewrite Ec1, Ec2.
-    apply mutrec_invariant_init; auto 10.
+    apply mrec_invariant_init; auto 10.
   - rewrite Ec1, Ec2. cbn.
-    rewrite unfold_interp_mutrec.
-    rewrite (unfold_bind (interp_mutrec _ _ d)).
+    rewrite unfold_interp_mrec.
+    rewrite (unfold_bind (interp_mrec _ _ d)).
     unfold observe, _observe; cbn.
     destruct (observe d); fold_observe; cbn.
-    + rewrite <- unfold_interp_mutrec.
-      apply mutrec_invariant_init; auto.
+    + rewrite <- unfold_interp_mrec.
+      apply mrec_invariant_init; auto.
     + pupto2_final; pfold; constructor; right.
       eapply self.
-      1: apply mutrec_bind; eassumption.
+      1: apply mrec_bind; eassumption.
       all: cbn; fold_bind; reflexivity.
     + destruct e; cbn.
       * fold_bind. rewrite <-bind_bind.
         pupto2_final. pfold. econstructor. right.
         eapply self.
-        1: apply mutrec_bind; eassumption.
+        1: apply mrec_bind; eassumption.
         all: cbn; reflexivity.
       * pupto2_final; pfold; constructor; right.
         eapply self.
-        1: apply mutrec_bind; eassumption.
+        1: apply mrec_bind; eassumption.
         all: cbn; fold_bind; reflexivity.
 Qed.
 
-Theorem interp_mutrec_is_interp : forall {T} (c : itree _ T),
-    eq_itree (interp_mutrec ctx _ c) (interp1 h_mutrec _ c).
+Theorem interp_mrec_is_interp : forall {T} (c : itree _ T),
+    eq_itree (interp_mrec ctx _ c) (interp1 h_mrec _ c).
 Proof.
-  intros; eapply mutrec_invariant_eq;
-    try eapply mutrec_main; reflexivity.
+  intros; eapply mrec_invariant_eq;
+    try eapply mrec_main; reflexivity.
 Qed.
 
 End Facts.
